AwsCryptographicMaterialProviders/runtimes/net/Generated/AwsCryptographyKeyStoreAdmin/InitializeMutationFlag.cs
@@ -1,0 +1,23 @@
+// Copyright Amazon.com Inc. or its affiliates. All Rights Reserved.
+// SPDX-License-Identifier: Apache-2.0
+// Do not modify this file. This file is machine generated, and any changes to it will be overwritten.
+using System;
+using AWS.Cryptography.KeyStoreAdmin;
+namespace AWS.Cryptography.KeyStoreAdmin
+{
+  using Amazon.Runtime;
+  public class InitializeMutationFlag : ConstantClass
+  {
+
+
+    public static readonly InitializeMutationFlag Created = new InitializeMutationFlag("Created");
+
+    public static readonly InitializeMutationFlag Resumed = new InitializeMutationFlag("Resumed");
+
+    public static readonly InitializeMutationFlag ResumedWithoutIndex = new InitializeMutationFlag("ResumedWithoutIndex");
+    public static readonly InitializeMutationFlag[] Values =  {
+ Created , Resumed , ResumedWithoutIndex
+};
+    public InitializeMutationFlag(string value) : base(value) { }
+  }
+}
