AwsCryptographicMaterialProviders/runtimes/python/src/aws_cryptographic_material_providers/smithygenerated/aws_cryptography_keystoreadmin/errors.py
@@ -1,0 +1,739 @@
+# Copyright Amazon.com Inc. or its affiliates. All Rights Reserved.
+# SPDX-License-Identifier: Apache-2.0
+# Do not modify this file. This file is machine generated, and any changes to it will be overwritten.
+
+import _dafny
+import aws_cryptographic_material_providers.internaldafny.generated
+import aws_cryptographic_material_providers.internaldafny.generated.AwsCryptographyKeyStoreAdminTypes
+from aws_cryptographic_material_providers.smithygenerated.aws_cryptography_keystore.errors import (
+    _smithy_error_to_dafny_error as aws_cryptography_keystore_smithy_error_to_dafny_error,
+)
+import aws_cryptographic_material_providers.smithygenerated.aws_cryptography_keystoreadmin.errors
+from aws_cryptography_internal_dynamodb.smithygenerated.com_amazonaws_dynamodb.shim import (
+    _sdk_error_to_dafny_error as com_amazonaws_dynamodb_sdk_error_to_dafny_error,
+)
+from aws_cryptography_internal_kms.smithygenerated.com_amazonaws_kms.shim import (
+    _sdk_error_to_dafny_error as com_amazonaws_kms_sdk_error_to_dafny_error,
+)
+from typing import Any, Dict, Generic, List, Literal, TypeVar
+
+
+class ServiceError(Exception):
+    """Base error for all errors in the service."""
+
+    pass
+
+
+T = TypeVar("T")
+
+
+class ApiError(ServiceError, Generic[T]):
+    """Base error for all api errors in the service."""
+
+    code: T
+
+    def __init__(self, message: str):
+        super().__init__(message)
+        self.message = message
+
+
+class UnknownApiError(ApiError[Literal["Unknown"]]):
+    """Error representing any unknown api errors."""
+
+    code: Literal["Unknown"] = "Unknown"
+
+
+class KeyStoreAdminException(ApiError[Literal["KeyStoreAdminException"]]):
+    code: Literal["KeyStoreAdminException"] = "KeyStoreAdminException"
+    message: str
+
+    def __init__(
+        self,
+        *,
+        message: str,
+    ):
+        super().__init__(message)
+
+    def as_dict(self) -> Dict[str, Any]:
+        """Converts the KeyStoreAdminException to a dictionary."""
+        return {
+            "message": self.message,
+            "code": self.code,
+        }
+
+    @staticmethod
+    def from_dict(d: Dict[str, Any]) -> "KeyStoreAdminException":
+        """Creates a KeyStoreAdminException from a dictionary."""
+        kwargs: Dict[str, Any] = {
+            "message": d["message"],
+        }
+
+        return KeyStoreAdminException(**kwargs)
+
+    def __repr__(self) -> str:
+        result = "KeyStoreAdminException("
+        if self.message is not None:
+            result += f"message={repr(self.message)}"
+
+        return result + ")"
+
+    def __eq__(self, other: Any) -> bool:
+        if not isinstance(other, KeyStoreAdminException):
+            return False
+        attributes: list[str] = [
+            "message",
+            "message",
+        ]
+        return all(getattr(self, a) == getattr(other, a) for a in attributes)
+
+
+class MutationFromException(ApiError[Literal["MutationFromException"]]):
+    code: Literal["MutationFromException"] = "MutationFromException"
+    message: str
+
+    def __init__(
+        self,
+        *,
+        message: str,
+    ):
+        """Key Management generic error encountered while mutating an item from
+        original to terminal.
+
+        Possibly, access to the terminal KMS Key was withdrawn.
+        :param message: A message associated with the specific error.
+        """
+        super().__init__(message)
+
+    def as_dict(self) -> Dict[str, Any]:
+        """Converts the MutationFromException to a dictionary."""
+        return {
+            "message": self.message,
+            "code": self.code,
+        }
+
+    @staticmethod
+    def from_dict(d: Dict[str, Any]) -> "MutationFromException":
+        """Creates a MutationFromException from a dictionary."""
+        kwargs: Dict[str, Any] = {
+            "message": d["message"],
+        }
+
+        return MutationFromException(**kwargs)
+
+    def __repr__(self) -> str:
+        result = "MutationFromException("
+        if self.message is not None:
+            result += f"message={repr(self.message)}"
+
+        return result + ")"
+
+    def __eq__(self, other: Any) -> bool:
+        if not isinstance(other, MutationFromException):
+            return False
+        attributes: list[str] = [
+            "message",
+            "message",
+        ]
+        return all(getattr(self, a) == getattr(other, a) for a in attributes)
+
+
+class MutationInvalidException(ApiError[Literal["MutationInvalidException"]]):
+    code: Literal["MutationInvalidException"] = "MutationInvalidException"
+    message: str
+
+    def __init__(
+        self,
+        *,
+        message: str,
+    ):
+        super().__init__(message)
+
+    def as_dict(self) -> Dict[str, Any]:
+        """Converts the MutationInvalidException to a dictionary."""
+        return {
+            "message": self.message,
+            "code": self.code,
+        }
+
+    @staticmethod
+    def from_dict(d: Dict[str, Any]) -> "MutationInvalidException":
+        """Creates a MutationInvalidException from a dictionary."""
+        kwargs: Dict[str, Any] = {
+            "message": d["message"],
+        }
+
+        return MutationInvalidException(**kwargs)
+
+    def __repr__(self) -> str:
+        result = "MutationInvalidException("
+        if self.message is not None:
+            result += f"message={repr(self.message)}"
+
+        return result + ")"
+
+    def __eq__(self, other: Any) -> bool:
+        if not isinstance(other, MutationInvalidException):
+            return False
+        attributes: list[str] = [
+            "message",
+            "message",
+        ]
+        return all(getattr(self, a) == getattr(other, a) for a in attributes)
+
+
+class MutationToException(ApiError[Literal["MutationToException"]]):
+    code: Literal["MutationToException"] = "MutationToException"
+    message: str
+
+    def __init__(
+        self,
+        *,
+        message: str,
+    ):
+        """Key Management generic error encountered while mutating an item from
+        original to terminal.
+
+        Possibly, access to the terminal KMS Key was withdrawn.
+        :param message: A message associated with the specific error.
+        """
+        super().__init__(message)
+
+    def as_dict(self) -> Dict[str, Any]:
+        """Converts the MutationToException to a dictionary."""
+        return {
+            "message": self.message,
+            "code": self.code,
+        }
+
+    @staticmethod
+    def from_dict(d: Dict[str, Any]) -> "MutationToException":
+        """Creates a MutationToException from a dictionary."""
+        kwargs: Dict[str, Any] = {
+            "message": d["message"],
+        }
+
+        return MutationToException(**kwargs)
+
+    def __repr__(self) -> str:
+        result = "MutationToException("
+        if self.message is not None:
+            result += f"message={repr(self.message)}"
+
+        return result + ")"
+
+    def __eq__(self, other: Any) -> bool:
+        if not isinstance(other, MutationToException):
+            return False
+        attributes: list[str] = [
+            "message",
+            "message",
+        ]
+        return all(getattr(self, a) == getattr(other, a) for a in attributes)
+
+
+class MutationVerificationException(ApiError[Literal["MutationVerificationException"]]):
+    code: Literal["MutationVerificationException"] = "MutationVerificationException"
+    message: str
+
+    def __init__(
+        self,
+        *,
+        message: str,
+    ):
+        """Key Management generic error encountered while authenticating an
+        item already in the terminal state.
+
+        Possibly, access to the terminal KMS Key was withdrawn.
+        :param message: A message associated with the specific error.
+        """
+        super().__init__(message)
+
+    def as_dict(self) -> Dict[str, Any]:
+        """Converts the MutationVerificationException to a dictionary."""
+        return {
+            "message": self.message,
+            "code": self.code,
+        }
+
+    @staticmethod
+    def from_dict(d: Dict[str, Any]) -> "MutationVerificationException":
+        """Creates a MutationVerificationException from a dictionary."""
+        kwargs: Dict[str, Any] = {
+            "message": d["message"],
+        }
+
+        return MutationVerificationException(**kwargs)
+
+    def __repr__(self) -> str:
+        result = "MutationVerificationException("
+        if self.message is not None:
+            result += f"message={repr(self.message)}"
+
+        return result + ")"
+
+    def __eq__(self, other: Any) -> bool:
+        if not isinstance(other, MutationVerificationException):
+            return False
+        attributes: list[str] = [
+            "message",
+            "message",
+        ]
+        return all(getattr(self, a) == getattr(other, a) for a in attributes)
+
+
+class UnexpectedStateException(ApiError[Literal["UnexpectedStateException"]]):
+    code: Literal["UnexpectedStateException"] = "UnexpectedStateException"
+    message: str
+
+    def __init__(
+        self,
+        *,
+        message: str,
+    ):
+        super().__init__(message)
+
+    def as_dict(self) -> Dict[str, Any]:
+        """Converts the UnexpectedStateException to a dictionary."""
+        return {
+            "message": self.message,
+            "code": self.code,
+        }
+
+    @staticmethod
+    def from_dict(d: Dict[str, Any]) -> "UnexpectedStateException":
+        """Creates a UnexpectedStateException from a dictionary."""
+        kwargs: Dict[str, Any] = {
+            "message": d["message"],
+        }
+
+        return UnexpectedStateException(**kwargs)
+
+    def __repr__(self) -> str:
+        result = "UnexpectedStateException("
+        if self.message is not None:
+            result += f"message={repr(self.message)}"
+
+        return result + ")"
+
+    def __eq__(self, other: Any) -> bool:
+        if not isinstance(other, UnexpectedStateException):
+            return False
+        attributes: list[str] = [
+            "message",
+            "message",
+        ]
+        return all(getattr(self, a) == getattr(other, a) for a in attributes)
+
+
+class UnsupportedFeatureException(ApiError[Literal["UnsupportedFeatureException"]]):
+    code: Literal["UnsupportedFeatureException"] = "UnsupportedFeatureException"
+    message: str
+
+    def __init__(
+        self,
+        *,
+        message: str,
+    ):
+        """This feature is not yet implemented.
+
+        :param message: A message associated with the specific error.
+        """
+        super().__init__(message)
+
+    def as_dict(self) -> Dict[str, Any]:
+        """Converts the UnsupportedFeatureException to a dictionary."""
+        return {
+            "message": self.message,
+            "code": self.code,
+        }
+
+    @staticmethod
+    def from_dict(d: Dict[str, Any]) -> "UnsupportedFeatureException":
+        """Creates a UnsupportedFeatureException from a dictionary."""
+        kwargs: Dict[str, Any] = {
+            "message": d["message"],
+        }
+
+        return UnsupportedFeatureException(**kwargs)
+
+    def __repr__(self) -> str:
+        result = "UnsupportedFeatureException("
+        if self.message is not None:
+            result += f"message={repr(self.message)}"
+
+        return result + ")"
+
+    def __eq__(self, other: Any) -> bool:
+        if not isinstance(other, UnsupportedFeatureException):
+            return False
+        attributes: list[str] = [
+            "message",
+            "message",
+        ]
+        return all(getattr(self, a) == getattr(other, a) for a in attributes)
+
+
+class MutationConflictException(ApiError[Literal["MutationConflictException"]]):
+    code: Literal["MutationConflictException"] = "MutationConflictException"
+    message: str
+
+    def __init__(
+        self,
+        *,
+        message: str,
+    ):
+        """A Mutation for this Branch Key ID is already inflight!
+
+        Nothing was changed. See <link>.
+        :param message: A message associated with the specific error.
+        """
+        super().__init__(message)
+
+    def as_dict(self) -> Dict[str, Any]:
+        """Converts the MutationConflictException to a dictionary."""
+        return {
+            "message": self.message,
+            "code": self.code,
+        }
+
+    @staticmethod
+    def from_dict(d: Dict[str, Any]) -> "MutationConflictException":
+        """Creates a MutationConflictException from a dictionary."""
+        kwargs: Dict[str, Any] = {
+            "message": d["message"],
+        }
+
+        return MutationConflictException(**kwargs)
+
+    def __repr__(self) -> str:
+        result = "MutationConflictException("
+        if self.message is not None:
+            result += f"message={repr(self.message)}"
+
+        return result + ")"
+
+    def __eq__(self, other: Any) -> bool:
+        if not isinstance(other, MutationConflictException):
+            return False
+        attributes: list[str] = [
+            "message",
+            "message",
+        ]
+        return all(getattr(self, a) == getattr(other, a) for a in attributes)
+
+
+class KeyStoreAdminException(ApiError[Literal["KeyStoreAdminException"]]):
+    code: Literal["KeyStoreAdminException"] = "KeyStoreAdminException"
+    message: str
+
+
+class MutationConflictException(ApiError[Literal["MutationConflictException"]]):
+    code: Literal["MutationConflictException"] = "MutationConflictException"
+    message: str
+
+
+class MutationFromException(ApiError[Literal["MutationFromException"]]):
+    code: Literal["MutationFromException"] = "MutationFromException"
+    message: str
+
+
+class MutationInvalidException(ApiError[Literal["MutationInvalidException"]]):
+    code: Literal["MutationInvalidException"] = "MutationInvalidException"
+    message: str
+
+
+class MutationToException(ApiError[Literal["MutationToException"]]):
+    code: Literal["MutationToException"] = "MutationToException"
+    message: str
+
+
+class MutationVerificationException(ApiError[Literal["MutationVerificationException"]]):
+    code: Literal["MutationVerificationException"] = "MutationVerificationException"
+    message: str
+
+
+class UnexpectedStateException(ApiError[Literal["UnexpectedStateException"]]):
+    code: Literal["UnexpectedStateException"] = "UnexpectedStateException"
+    message: str
+
+
+class UnsupportedFeatureException(ApiError[Literal["UnsupportedFeatureException"]]):
+    code: Literal["UnsupportedFeatureException"] = "UnsupportedFeatureException"
+    message: str
+
+
+class ComAmazonawsDynamodb(ApiError[Literal["ComAmazonawsDynamodb"]]):
+    ComAmazonawsDynamodb: Any
+
+
+class ComAmazonawsKms(ApiError[Literal["ComAmazonawsKms"]]):
+    ComAmazonawsKms: Any
+
+
+class KeyStore(ApiError[Literal["KeyStore"]]):
+    KeyStore: Any
+
+
+class CollectionOfErrors(ApiError[Literal["CollectionOfErrors"]]):
+    code: Literal["CollectionOfErrors"] = "CollectionOfErrors"
+    message: str
+    list: List[ServiceError]
+
+    def __init__(self, *, message: str, list):
+        super().__init__(message)
+        self.list = list
+
+    def as_dict(self) -> Dict[str, Any]:
+        """Converts the CollectionOfErrors to a dictionary.
+
+        The dictionary uses the modeled shape names rather than the
+        parameter names as keys to be mostly compatible with boto3.
+        """
+        return {
+            "message": self.message,
+            "code": self.code,
+            "list": self.list,
+        }
+
+    @staticmethod
+    def from_dict(d: Dict[str, Any]) -> "CollectionOfErrors":
+        """Creates a CollectionOfErrors from a dictionary.
+
+        The dictionary is expected to use the modeled shape names rather
+        than the parameter names as keys to be mostly compatible with
+        boto3.
+        """
+        kwargs: Dict[str, Any] = {"message": d["message"], "list": d["list"]}
+
+        return CollectionOfErrors(**kwargs)
+
+    def __repr__(self) -> str:
+        result = "CollectionOfErrors("
+        result += f"message={self.message},"
+        if self.message is not None:
+            result += f"message={repr(self.message)}"
+        result += f"list={self.list}"
+        result += ")"
+        return result
+
+    def __eq__(self, other: Any) -> bool:
+        if not isinstance(other, CollectionOfErrors):
+            return False
+        if not (self.list == other.list):
+            return False
+        attributes: list[str] = ["message", "message"]
+        return all(getattr(self, a) == getattr(other, a) for a in attributes)
+
+
+class OpaqueError(ApiError[Literal["OpaqueError"]]):
+    code: Literal["OpaqueError"] = "OpaqueError"
+    obj: Any  # As an OpaqueError, type of obj is unknown
+
+    def __init__(self, *, obj):
+        super().__init__("")
+        self.obj = obj
+
+    def as_dict(self) -> Dict[str, Any]:
+        """Converts the OpaqueError to a dictionary.
+
+        The dictionary uses the modeled shape names rather than the
+        parameter names as keys to be mostly compatible with boto3.
+        """
+        return {
+            "message": self.message,
+            "code": self.code,
+            "obj": self.obj,
+        }
+
+    @staticmethod
+    def from_dict(d: Dict[str, Any]) -> "OpaqueError":
+        """Creates a OpaqueError from a dictionary.
+
+        The dictionary is expected to use the modeled shape names rather
+        than the parameter names as keys to be mostly compatible with
+        boto3.
+        """
+        kwargs: Dict[str, Any] = {"message": d["message"], "obj": d["obj"]}
+
+        return OpaqueError(**kwargs)
+
+    def __repr__(self) -> str:
+        result = "OpaqueError("
+        result += f"message={self.message},"
+        if self.message is not None:
+            result += f"message={repr(self.message)}"
+        result += f"obj={self.obj}"
+        result += ")"
+        return result
+
+    def __eq__(self, other: Any) -> bool:
+        if not isinstance(other, OpaqueError):
+            return False
+        if not (self.obj == other.obj):
+            return False
+        attributes: list[str] = ["message", "message"]
+        return all(getattr(self, a) == getattr(other, a) for a in attributes)
+
+
+class OpaqueWithTextError(ApiError[Literal["OpaqueWithTextError"]]):
+    code: Literal["OpaqueWithTextError"] = "OpaqueWithTextError"
+    obj: Any  # As an OpaqueWithTextError, type of obj is unknown
+    obj_message: str  # obj_message is a message representing the details of obj
+
+    def __init__(self, *, obj, obj_message):
+        super().__init__("")
+        self.obj = obj
+        self.obj_message = obj_message
+
+    def as_dict(self) -> Dict[str, Any]:
+        """Converts the OpaqueWithTextError to a dictionary.
+
+        The dictionary uses the modeled shape names rather than the
+        parameter names as keys to be mostly compatible with boto3.
+        """
+        return {
+            "message": self.message,
+            "code": self.code,
+            "obj": self.obj,
+            "obj_message": self.obj_message,
+        }
+
+    @staticmethod
+    def from_dict(d: Dict[str, Any]) -> "OpaqueWithTextError":
+        """Creates a OpaqueWithTextError from a dictionary.
+
+        The dictionary is expected to use the modeled shape names rather
+        than the parameter names as keys to be mostly compatible with
+        boto3.
+        """
+        kwargs: Dict[str, Any] = {
+            "message": d["message"],
+            "obj": d["obj"],
+            "obj_message": d["obj_message"],
+        }
+
+        return OpaqueWithTextError(**kwargs)
+
+    def __repr__(self) -> str:
+        result = "OpaqueWithTextError("
+        result += f"message={self.message},"
+        if self.message is not None:
+            result += f"message={repr(self.message)}"
+        result += f"obj={self.obj}"
+        result += f"obj_message={self.obj_message}"
+        result += ")"
+        return result
+
+    def __eq__(self, other: Any) -> bool:
+        if not isinstance(other, OpaqueWithTextError):
+            return False
+        if not (self.obj == other.obj):
+            return False
+        attributes: list[str] = ["message", "message"]
+        return all(getattr(self, a) == getattr(other, a) for a in attributes)
+
+
+def _smithy_error_to_dafny_error(e: ServiceError):
+    """Converts the provided native Smithy-modeled error into the corresponding
+    Dafny error."""
+    if isinstance(
+        e,
+        aws_cryptographic_material_providers.smithygenerated.aws_cryptography_keystoreadmin.errors.KeyStoreAdminException,
+    ):
+        return aws_cryptographic_material_providers.internaldafny.generated.AwsCryptographyKeyStoreAdminTypes.Error_KeyStoreAdminException(
+            message=_dafny.Seq(e.message)
+        )
+
+    if isinstance(
+        e,
+        aws_cryptographic_material_providers.smithygenerated.aws_cryptography_keystoreadmin.errors.MutationConflictException,
+    ):
+        return aws_cryptographic_material_providers.internaldafny.generated.AwsCryptographyKeyStoreAdminTypes.Error_MutationConflictException(
+            message=_dafny.Seq(e.message)
+        )
+
+    if isinstance(
+        e,
+        aws_cryptographic_material_providers.smithygenerated.aws_cryptography_keystoreadmin.errors.MutationFromException,
+    ):
+        return aws_cryptographic_material_providers.internaldafny.generated.AwsCryptographyKeyStoreAdminTypes.Error_MutationFromException(
+            message=_dafny.Seq(e.message)
+        )
+
+    if isinstance(
+        e,
+        aws_cryptographic_material_providers.smithygenerated.aws_cryptography_keystoreadmin.errors.MutationInvalidException,
+    ):
+        return aws_cryptographic_material_providers.internaldafny.generated.AwsCryptographyKeyStoreAdminTypes.Error_MutationInvalidException(
+            message=_dafny.Seq(e.message)
+        )
+
+    if isinstance(
+        e,
+        aws_cryptographic_material_providers.smithygenerated.aws_cryptography_keystoreadmin.errors.MutationToException,
+    ):
+        return aws_cryptographic_material_providers.internaldafny.generated.AwsCryptographyKeyStoreAdminTypes.Error_MutationToException(
+            message=_dafny.Seq(e.message)
+        )
+
+    if isinstance(
+        e,
+        aws_cryptographic_material_providers.smithygenerated.aws_cryptography_keystoreadmin.errors.MutationVerificationException,
+    ):
+        return aws_cryptographic_material_providers.internaldafny.generated.AwsCryptographyKeyStoreAdminTypes.Error_MutationVerificationException(
+            message=_dafny.Seq(e.message)
+        )
+
+    if isinstance(
+        e,
+        aws_cryptographic_material_providers.smithygenerated.aws_cryptography_keystoreadmin.errors.UnexpectedStateException,
+    ):
+        return aws_cryptographic_material_providers.internaldafny.generated.AwsCryptographyKeyStoreAdminTypes.Error_UnexpectedStateException(
+            message=_dafny.Seq(e.message)
+        )
+
+    if isinstance(
+        e,
+        aws_cryptographic_material_providers.smithygenerated.aws_cryptography_keystoreadmin.errors.UnsupportedFeatureException,
+    ):
+        return aws_cryptographic_material_providers.internaldafny.generated.AwsCryptographyKeyStoreAdminTypes.Error_UnsupportedFeatureException(
+            message=_dafny.Seq(e.message)
+        )
+
+    if isinstance(e, ComAmazonawsDynamodb):
+        return aws_cryptographic_material_providers.internaldafny.generated.AwsCryptographyKeyStoreAdminTypes.Error_ComAmazonawsDynamodb(
+            com_amazonaws_dynamodb_sdk_error_to_dafny_error(e.message)
+        )
+
+    if isinstance(e, ComAmazonawsKms):
+        return aws_cryptographic_material_providers.internaldafny.generated.AwsCryptographyKeyStoreAdminTypes.Error_ComAmazonawsKms(
+            com_amazonaws_kms_sdk_error_to_dafny_error(e.message)
+        )
+
+    if isinstance(e, KeyStore):
+        return aws_cryptographic_material_providers.internaldafny.generated.AwsCryptographyKeyStoreAdminTypes.Error_AwsCryptographyKeyStore(
+            aws_cryptography_keystore_smithy_error_to_dafny_error(e.message)
+        )
+
+    if isinstance(e, CollectionOfErrors):
+        return aws_cryptographic_material_providers.internaldafny.generated.AwsCryptographyKeyStoreAdminTypes.Error_CollectionOfErrors(
+            message=_dafny.Seq(e.message),
+            list=_dafny.Seq(
+                _smithy_error_to_dafny_error(native_err) for native_err in e.list
+            ),
+        )
+
+    if isinstance(e, OpaqueError):
+        return aws_cryptographic_material_providers.internaldafny.generated.AwsCryptographyKeyStoreAdminTypes.Error_Opaque(
+            obj=e.obj
+        )
+
+    if isinstance(e, OpaqueWithTextError):
+        return aws_cryptographic_material_providers.internaldafny.generated.AwsCryptographyKeyStoreAdminTypes.Error_OpaqueWithText(
+            obj=e.obj, objMessage=e.obj_message
+        )
+
+    else:
+        return aws_cryptographic_material_providers.internaldafny.generated.AwsCryptographyKeyStoreAdminTypes.Error_Opaque(
+            obj=e
+        )
