AwsCryptographicMaterialProviders/dafny/AwsCryptographyKeyStoreAdmin/src/MutationStateStructures.dfy
@@ -1,0 +1,499 @@
+// Copyright Amazon.com Inc. or its affiliates. All Rights Reserved.
+// SPDX-License-Identifier: Apache-2.0
+include "../Model/AwsCryptographyKeyStoreAdminTypes.dfy"
+include "../../../../libraries/src/Collections/Sets/Sets.dfy"
+include "../../../../libraries/src/Collections/Maps/Maps.dfy"
+include "../../../../libraries/src/JSON/API.dfy"
+include "../../../../libraries/src/JSON/Errors.dfy"
+include "../../../../libraries/src/JSON/Values.dfy"
+include "MutationIndexUtils.dfy"
+
+/** Mutation State Structures describe the Mutable Branch Key Properties that can be changed by Mutaiton. **/
+/** Methods here normialize these descriptions so they may be compared. **/
+module {:options "/functionSyntax:4" } MutationStateStructures {
+  import opened StandardLibrary
+  import opened StandardLibrary.UInt
+  import opened Wrappers
+  import opened Seq
+  import UTF8
+  import String = StandardLibrary.String
+  import Sets
+  import Maps
+  import SortedSets
+
+  import ErrorMessages = KeyStoreErrorMessages
+  import Types = AwsCryptographyKeyStoreAdminTypes
+  import KeyStoreOperations = AwsCryptographyKeyStoreOperations
+  import KeyStoreTypes = KeyStoreOperations.Types
+  import KmsArn
+  import Structure
+
+  import JSON = JSON.API
+  import JSONErrors = JSON.Errors
+  import JSONValues = JSON.Values
+  import MutationIndexUtils
+
+  const MUTABLE_PROPERTY_COUNT: int := 2
+  const MUTABLE_PROPERTY_COUNT_str := "2"
+  const AWS_CRYPTO_EC := Structure.AWS_CRYPTO_EC
+  const KMS_FIELD := Structure.KMS_FIELD
+  // Ensures
+  // - if KMS ARN, Valid KMS ARN
+  // - if EC, Valid non-empty EC, & not restricted field names
+  // - non-empty
+  predicate ValidMutations?(
+    input: Types.Mutations
+  )
+  {
+    && (input.TerminalKmsArn.Some? ==> KmsArn.ValidKmsArn?(input.TerminalKmsArn.value))
+    && (input.TerminalEncryptionContext.Some? ==>
+          && |input.TerminalEncryptionContext.value| > 0
+          &&  forall k <- input.TerminalEncryptionContext.value ::
+               && |k| > 0 && |input.TerminalEncryptionContext.value[k]| > 0
+               && input.TerminalEncryptionContext.value.Keys !! Structure.BRANCH_KEY_RESTRICTED_FIELD_NAMES)
+    && !(input.TerminalKmsArn.None? && input.TerminalEncryptionContext.None?)
+  }
+
+  datatype MutableProperties = | MutableProperties (
+    nameonly kmsArn: validKmsArn,
+    nameonly customEncryptionContext: KeyStoreTypes.EncryptionContextString
+  )
+
+  type validKmsArn = s:string | KmsArn.ValidKmsArn?(s) witness *
+
+  datatype MutationToApply = | MutationToApply(
+    Identifier: string,
+    Original: MutableProperties,
+    Terminal: MutableProperties,
+    CreateTime: string,
+    ExclusiveStartKey: MutationIndexUtils.ExclusiveStartKey := Option.None,
+    UUID: string,
+    Input: Types.Mutations,
+    CommitmentCiphertext: seq<uint8>,
+    IndexCiphertext: seq<uint8>
+  )
+
+  /** The Commitment & Index are persisted to the storage by Initialize. **/
+  /** The Commitment & Index are read by Apply. **/
+  /** The Index is updated by Apply. **/
+  /** Both are deleted when the Mutation is completed by Apply. **/
+  datatype CommitmentAndIndex = CommitmentAndIndex(
+    Commitment: KeyStoreTypes.MutationCommitment,
+    Index: KeyStoreTypes.MutationIndex
+  )
+  {
+    /** The Commitment & Index MUST always have the same Identifier & UUID. **/
+    /** They MAY NOT have the same CreateTime. **/
+    ghost predicate ValidState()
+    {
+      && Commitment.Identifier == Index.Identifier
+      && Commitment.UUID == Index.UUID
+    }
+  }
+
+  predicate MutationToApply?(MutationToApply: MutationToApply)
+  {
+    && KmsArn.ValidKmsArn?(MutationToApply.Original.kmsArn)
+    && KmsArn.ValidKmsArn?(MutationToApply.Terminal.kmsArn)
+    && (Structure.BRANCH_KEY_RESTRICTED_FIELD_NAMES !! MutationToApply.Original.customEncryptionContext.Keys)
+    && (Structure.BRANCH_KEY_RESTRICTED_FIELD_NAMES !! MutationToApply.Terminal.customEncryptionContext.Keys)
+  }
+
+  function EncryptionContextStringToJSON(
+    encryptionContext: KeyStoreTypes.EncryptionContextString
+  ): (output: JSONValues.JSON)
+
+  {
+    var keys := SortedSets.ComputeSetToOrderedSequence2(encryptionContext.Keys, (a, b) => a < b);
+
+    if |keys| == 0 then
+      JSONValues.Object([])
+    else
+      var KeysAndValues
+        := Seq.Map(
+             k
+             requires k in encryptionContext
+             => (k, JSONValues.JSON.String(encryptionContext[k]))
+           , keys);
+      JSONValues.Object(KeysAndValues)
+  }
+
+  function JSONToEncryptionContextString(
+    EncryptionContext: JSONValues.JSON
+  ): (output: KeyStoreTypes.EncryptionContextString)
+    requires EncryptionContext.Object?
+    requires forall p <- EncryptionContext.obj :: p.1.String?
+    requires |set p <- EncryptionContext.obj :: p.0| == |EncryptionContext.obj|
+  {
+    LemmaJSONObjectCanConvertToDafnyMap(EncryptionContext);
+    map
+      i | 0 <= i < |EncryptionContext.obj|
+      ::
+        EncryptionContext.obj[i].0 := EncryptionContext.obj[i].1.str
+  }
+
+  function KmsArnToJSON(
+    kmsArn: string
+  ): (output: Result<JSONValues.JSON, Types.Error>)
+  {
+    Success(JSONValues.JSON.String(kmsArn))
+  }
+
+  function NeedOutcome<E>(
+    condition: bool,
+    error: () --> E)
+    : (result: Outcome2<E>)
+    requires !condition ==> error.requires()
+  {
+    if condition then Outcome2.Pass else Outcome2.Fail(error())
+  }
+
+  datatype Outcome2<E> = Pass | Fail(error: E)
+  {
+    predicate IsFailure() {
+      Fail?
+    }
+    // Note: PropagateFailure returns a Result, not an Outcome.
+    function PropagateFailure(): Outcome<E>
+      requires Fail?
+    {
+      Outcome.Fail(this.error)
+    }
+    // Note: no Extract method
+  }
+
+  function InputMutationsToJson(
+    Mutations: Types.Mutations
+  ): (output: JSONValues.JSON)
+  {
+    var ec: JSONValues.JSON :=
+      if Mutations.TerminalEncryptionContext.Some?
+      then EncryptionContextStringToJSON(Mutations.TerminalEncryptionContext.value)
+      else JSONValues.Null;
+    var kms: JSONValues.JSON :=
+      if Mutations.TerminalKmsArn.Some?
+      then JSONValues.JSON.String(Mutations.TerminalKmsArn.value)
+      else JSONValues.Null;
+    var inputJson
+      := JSONValues.Object([(AWS_CRYPTO_EC, ec), (KMS_FIELD, kms)]);
+    inputJson
+  }
+
+  function InputMutationsFromJson(
+    MutationsJson: JSONValues.JSON
+  ): (output: Types.Mutations)
+    requires MutationsJson.Object? && |MutationsJson.obj| == 2
+    requires MutationsJson.obj[0].1.Object? ==>
+               (var EncryptionContext := MutationsJson.obj[0].1;
+                && (forall p <- EncryptionContext.obj :: p.1.String?)
+                && (|set p <- EncryptionContext.obj :: p.0| == |EncryptionContext.obj|))
+  {
+    var ec: Option<KeyStoreTypes.EncryptionContextString> :=
+      if MutationsJson.obj[0].1.Object?
+      then Some(JSONToEncryptionContextString(MutationsJson.obj[0].1))
+      else None;
+    var kms: Option<string> :=
+      if MutationsJson.obj[1].1.String?
+      then Some(MutationsJson.obj[1].1.str)
+      else None;
+    var input
+      := Types.Mutations(
+           TerminalKmsArn := kms,
+           TerminalEncryptionContext := ec);
+    input
+  }
+
+  function DeserializeMutationInput(
+    commitment: KeyStoreTypes.MutationCommitment
+  ): (output: Result<Types.Mutations, Types.Error>)
+  {
+    var InputJson :- JSON.Deserialize(commitment.Input).MapFailure(
+                       (e: JSONErrors.DeserializationError)
+                       => Types.KeyStoreAdminException(
+                           message := "Could not JSON Deserialize: Input. " + e.ToString()));
+    :- MutationsInputJson?(InputJson);
+    var input := InputMutationsFromJson(InputJson);
+    Success(input)
+  }
+
+  function SerializeMutationCommitment(
+    MutationToApply: MutationToApply
+  ): (output: Result<KeyStoreTypes.MutationCommitment, Types.Error>)
+    requires MutationToApply?(MutationToApply)
+  {
+    var OriginalJson
+      := JSONValues.Object(
+           [
+             (AWS_CRYPTO_EC, EncryptionContextStringToJSON(MutationToApply.Original.customEncryptionContext)),
+             (KMS_FIELD, JSONValues.JSON.String(MutationToApply.Original.kmsArn))
+           ]);
+    var TerminalJson
+      := JSONValues.Object(
+           [
+             (AWS_CRYPTO_EC, EncryptionContextStringToJSON(MutationToApply.Terminal.customEncryptionContext)),
+             (KMS_FIELD, JSONValues.JSON.String(MutationToApply.Terminal.kmsArn))
+           ]);
+
+    var InputJson := InputMutationsToJson(MutationToApply.Input);
+
+    var originalBytes :- JSON.Serialize(OriginalJson).MapFailure(
+                           (e: JSONErrors.SerializationError)
+                           => Types.KeyStoreAdminException(
+                               message := "Could not JSON Serialize state: original properties. " + e.ToString()));
+    var terminalBytes :- JSON.Serialize(TerminalJson).MapFailure(
+                           (e: JSONErrors.SerializationError)
+                           => Types.KeyStoreAdminException(
+                               message := "Could not JSON Serialize state: terminal properties. " + e.ToString()));
+    var inputBytes :- JSON.Serialize(InputJson).MapFailure(
+                        (e: JSONErrors.SerializationError)
+                        => Types.KeyStoreAdminException(
+                            message := "Could not JSON Serialize Input. " + e.ToString()));
+    var commitment := KeyStoreTypes.MutationCommitment(
+                        Identifier := MutationToApply.Identifier,
+                        Original := originalBytes,
+                        Terminal := terminalBytes,
+                        UUID := MutationToApply.UUID,
+                        CreateTime := MutationToApply.CreateTime,
+                        CiphertextBlob := MutationToApply.CommitmentCiphertext,
+                        Input := inputBytes
+                      );
+    Success(commitment)
+  }
+
+  function SerializeMutationIndex(
+    MutationToApply: MutationToApply,
+    ExclusiveStartKey: MutationIndexUtils.ExclusiveStartKey
+  ): (output: Result<KeyStoreTypes.MutationIndex, Types.Error>)
+    requires MutationToApply?(MutationToApply)
+  {
+    var index := KeyStoreTypes.MutationIndex(
+                   Identifier := MutationToApply.Identifier,
+                   PageIndex := MutationIndexUtils.ExclusiveStartKeyToPageIndex(ExclusiveStartKey),
+                   UUID := MutationToApply.UUID,
+                   CreateTime := MutationToApply.CreateTime,
+                   CiphertextBlob := MutationToApply.IndexCiphertext // TODO-Mutations-GA
+                 );
+    Success(index)
+  }
+
+  function DeserializeMutation(
+    commitmentAndIndex: CommitmentAndIndex
+  ): (output: Result<MutationToApply, Types.Error>)
+    ensures output.Success? ==> MutationToApply?(output.value)
+  {
+    var commitment := commitmentAndIndex.Commitment;
+    var index := commitmentAndIndex.Index;
+    var OriginalJson :- JSON.Deserialize(commitment.Original).MapFailure(
+                          (e: JSONErrors.DeserializationError)
+                          => Types.KeyStoreAdminException(
+                              message := "Could not JSON Deserialize: original properties. " + e.ToString()));
+
+    var TerminalJson :- JSON.Deserialize(commitment.Terminal).MapFailure(
+                          (e: JSONErrors.DeserializationError)
+                          => Types.KeyStoreAdminException(
+                              message := "Could not JSON Deserialize: terminal properties. " + e.ToString()));
+    var InputJson :- JSON.Deserialize(commitment.Input).MapFailure(
+                       (e: JSONErrors.DeserializationError)
+                       => Types.KeyStoreAdminException(
+                           message := "Could not JSON Deserialize: Input. " + e.ToString()));
+
+    :- MutablePropertiesJson?(OriginalJson);
+    :- MutablePropertiesJson?(TerminalJson);
+    :- MutationsInputJson?(InputJson);
+
+    Success(
+      MutationToApply(
+        Identifier := commitment.Identifier,
+        Original := MutableProperties(
+          kmsArn := OriginalJson.obj[1].1.str,
+          customEncryptionContext := JSONToEncryptionContextString(OriginalJson.obj[0].1)
+        ),
+        Terminal := MutableProperties(
+          kmsArn := TerminalJson.obj[1].1.str,
+          customEncryptionContext := JSONToEncryptionContextString(TerminalJson.obj[0].1)
+        ),
+        UUID := commitment.UUID,
+        CreateTime := commitment.CreateTime,
+        ExclusiveStartKey := MutationIndexUtils.PageIndexToExclusiveStartKey(index.PageIndex),
+        CommitmentCiphertext := commitment.CiphertextBlob,
+        IndexCiphertext := index.CiphertextBlob,
+        Input := InputMutationsFromJson(InputJson)
+      ))
+  }
+
+  const ERROR_PRFX := "Serialized State properties is malformed! "
+
+  function MutablePropertiesJson?(
+    MutableProperties: JSONValues.JSON
+  ): (output: Outcome<Types.Error>)
+  {
+    :- NeedOutcome(
+         MutableProperties.Object? && |MutableProperties.obj| == 2,
+         () => Types.KeyStoreAdminException( message := ERROR_PRFX + "There should be two objects.")
+       );
+    :- NeedOutcome(
+         MutableProperties.obj[0].0 == AWS_CRYPTO_EC,
+         () => Types.KeyStoreAdminException( message := ERROR_PRFX + "First Key MUST be Encryption Context.")
+       );
+    :- NeedOutcome(
+         MutableProperties.obj[1].0 == KMS_FIELD,
+         () => Types.KeyStoreAdminException( message := ERROR_PRFX + "Second Key MUST be KMS ARN.")
+       );
+    :- NeedOutcome(
+         MutableProperties.obj[0].1.Object?,
+         () => Types.KeyStoreAdminException(
+             message := ERROR_PRFX + "Value for `" + AWS_CRYPTO_EC + "` MUST be an object.")
+       );
+    :- NeedOutcome(
+         MutableProperties.obj[1].1.String?,
+         () => Types.KeyStoreAdminException(
+             message := ERROR_PRFX + "Value for `" + KMS_FIELD + "` MUST be a string.")
+       );
+    :- NeedOutcome(
+         KmsArn.ValidKmsArn?(MutableProperties.obj[1].1.str),
+         () => Types.KeyStoreAdminException( message := ERROR_PRFX + "KMS ARN that has been deserialized is invalid.")
+       );
+
+    var EncryptionContext := MutableProperties.obj[0].1;
+    :- NeedOutcome(
+         forall p <- EncryptionContext.obj :: p.1.String?,
+         () => Types.KeyStoreAdminException( message := ERROR_PRFX + "Member of Encryption Context cannot be deserialized.")
+       );
+
+    var EncryptionContextKeys := set p <- EncryptionContext.obj :: p.0;
+    :- NeedOutcome(
+         |EncryptionContextKeys| == |EncryptionContext.obj|,
+         () => Types.KeyStoreAdminException(
+             message := ERROR_PRFX + "Size of Encryption Context keys is not equal to size of Encryption Context values. ")
+       );
+
+    :- NeedOutcome(
+         Structure.BRANCH_KEY_RESTRICTED_FIELD_NAMES !! EncryptionContextKeys,
+         () => Types.KeyStoreAdminException(
+             message := "Invalid Mutation Token: MUST NOT model Item specific fields!"
+           )
+       );
+
+    Outcome.Pass
+  }
+
+  function MutationsInputJson?(
+    DeserializedMutations: JSONValues.JSON
+  ): (output: Outcome<Types.Error>)
+  {
+    :- NeedOutcome(
+         DeserializedMutations.Object? && |DeserializedMutations.obj| == 2,
+         () => Types.KeyStoreAdminException( message := ERROR_PRFX + "There MUST not be more than two objects.")
+       );
+    :- NeedOutcome(
+         DeserializedMutations.obj[0].0 == AWS_CRYPTO_EC,
+         () => Types.KeyStoreAdminException( message := ERROR_PRFX + "First Key MUST be Encryption Context.")
+       );
+    :- NeedOutcome(
+         DeserializedMutations.obj[1].0 == KMS_FIELD,
+         () => Types.KeyStoreAdminException( message := ERROR_PRFX + "Second Key MUST be KMS ARN.")
+       );
+    :- NeedOutcome(
+         DeserializedMutations.obj[0].1.Object? || DeserializedMutations.obj[0].1.Null?,
+         () => Types.KeyStoreAdminException(
+             message := ERROR_PRFX + "Value for `" + AWS_CRYPTO_EC + "` MUST be an object or Null.")
+       );
+    :- NeedOutcome(
+         DeserializedMutations.obj[1].1.String? || DeserializedMutations.obj[1].1.Null?,
+         () => Types.KeyStoreAdminException(
+             message := ERROR_PRFX + "Value for `" + KMS_FIELD + "` MUST be a string or Null.")
+       );
+
+    // For the input, I do not think we care if the KMS ARN is valid
+    // :- NeedOutcome(
+    //      KmsArn.ValidKmsArn?(DeserializedMutations.obj[1].1.str),
+    //      () => Types.KeyStoreAdminException( message := ERROR_PRFX + "KMS ARN that has been deserialized is invalid.")
+    //    );
+    NullableEncryptionContextJson?(DeserializedMutations.obj[0].1)
+  }
+
+  function NullableEncryptionContextJson?(
+    NullableEncryptionContext: JSONValues.JSON
+  ): (output: Outcome<Types.Error>)
+    requires NullableEncryptionContext.Object? || NullableEncryptionContext.Null?
+  {
+    if NullableEncryptionContext.Null?
+    then Outcome.Pass
+    else EncryptionContextJson?(NullableEncryptionContext)
+  }
+
+  function EncryptionContextJson?(
+    EncryptionContextJson: JSONValues.JSON
+  ): (output: Outcome<Types.Error>)
+    requires EncryptionContextJson.Object?
+  {
+    :- NeedOutcome(
+         forall p <- EncryptionContextJson.obj :: p.1.String?,
+         () => Types.KeyStoreAdminException( message := ERROR_PRFX + "Member of Encryption Context cannot be deserialized.")
+       );
+
+    var EncryptionContextKeys := set p <- EncryptionContextJson.obj :: p.0;
+    :- NeedOutcome(
+         |EncryptionContextKeys| == |EncryptionContextJson.obj|,
+         () => Types.KeyStoreAdminException(
+             message := ERROR_PRFX + "Size of Encryption Context keys is not equal to size of Encryption Context values. ")
+       );
+    :- NeedOutcome(
+         Structure.BRANCH_KEY_RESTRICTED_FIELD_NAMES !! EncryptionContextKeys,
+         () => Types.KeyStoreAdminException(
+             message := "Invalid Mutation Token: MUST NOT model Item specific fields!")
+       );
+    Outcome.Pass
+  }
+
+  // Quality of life proof that a correctly constructed JSON object,
+  // will in fact go into a Dafny Map
+  lemma LemmaJSONObjectCanConvertToDafnyMap(
+    Object: JSONValues.JSON
+  )
+    requires Object.Object?
+    requires |JSONObjectKeysToSet(Object)| == |Object.obj|
+    decreases |Object.obj|
+    ensures
+      && (forall i, j
+            :: 0 <= i < j < |Object.obj|
+               ==> Object.obj[i].0 != Object.obj[j].0)
+  {
+    if |Object.obj| == 0 {
+    } else {
+      assert Object.obj == [Seq.First(Object.obj)] + Seq.DropFirst(Object.obj);
+      assert JSONObjectKeysToSet(Object) == {First(Object.obj).0} + JSONObjectKeysToSet(JSONValues.Object(DropFirst(Object.obj)));
+      if First(Object.obj) in DropFirst(Object.obj) {
+        //   // If there is a duplicate, then we show that |JSONObjectKeysToSet(s)| == |s| cannot hold.
+        assert JSONObjectKeysToSet(Object) == JSONObjectKeysToSet(JSONValues.Object(DropFirst(Object.obj)));
+        LemmaCardinalityOfSet(JSONValues.Object(DropFirst(Object.obj)));
+        assert |JSONObjectKeysToSet(Object)| <= |DropFirst(Object.obj)|;
+      } else {
+        LemmaCardinalityOfSet(JSONValues.Object(DropFirst(Object.obj)));
+        assert |JSONObjectKeysToSet(Object)| == 1 + |JSONObjectKeysToSet(JSONValues.Object(DropFirst(Object.obj)))|;
+        LemmaJSONObjectCanConvertToDafnyMap(JSONValues.Object(DropFirst(Object.obj)));
+      }
+    }
+  }
+
+  function JSONObjectKeysToSet(
+    Object: JSONValues.JSON
+  ): (output: set<string>)
+    requires Object.Object?
+  {
+    set p <- Object.obj :: p.0
+  }
+
+  lemma LemmaCardinalityOfSet(Object: JSONValues.JSON)
+    requires Object.Object?
+    decreases |Object.obj|
+    ensures |JSONObjectKeysToSet(Object)| <= |Object.obj|
+  {
+    if |Object.obj| == 0 {
+    } else {
+      assert JSONObjectKeysToSet(Object)
+          == JSONObjectKeysToSet(JSONValues.Object(DropLast(Object.obj))) + {Last(Object.obj).0};
+      LemmaCardinalityOfSet(JSONValues.Object(DropLast(Object.obj)));
+    }
+  }
+}
